src/lib/communication/DY.Lib.Communication.RequestResponse.Lemmas.fst
@@ -80,6 +80,9 @@ instance parseable_serializeable_bytes_state_id: parseable_serializeable bytes s
 instance parseable_serializeable_bytes_principal: parseable_serializeable bytes principal
   = mk_parseable_serializeable ps_principal
 
+instance parseable_serializeable_bytes_option (a:Type0) {|ps_a:parser_serializer bytes a|}: parseable_serializeable bytes (option a)
+  = mk_parseable_serializeable (ps_option ps_a)
+
 val comm_meta_data_knowable_proof: 
   {|crypto_invariants|} ->
   tr:trace ->
@@ -102,6 +105,9 @@ let comm_meta_data_knowable_proof #cinvs tr a #ps st_t #ps_st_t sess_id st #loca
   );
   assert(is_well_formed state_id (is_knowable_by lab tr) req_meta_data.sid);
   assert(is_well_formed principal (is_knowable_by lab tr) req_meta_data.server);
+  match req_meta_data.client with
+  | None -> ()
+  | Some client -> assert(is_well_formed principal (is_knowable_by lab tr) client);
   ()
 
 val comm_client_state_invariant: 
@@ -112,7 +118,7 @@ val comm_client_state_invariant:
   prop
 let comm_client_state_invariant #cinvs tr a #ps prin req_meta_data =
   comm_meta_data_knowable tr a prin req_meta_data /\
-  event_triggered tr prin (CommClientSendRequest prin req_meta_data.server req_meta_data.request req_meta_data.key <: communication_reqres_event a)
+  event_triggered tr prin (CommClientSendRequest (Some? req_meta_data.client) prin req_meta_data.server req_meta_data.request req_meta_data.key <: communication_reqres_event a)
 
 /// The communication layer makes use of many lemmas with SMT patterns.
 /// These lemmas depend, however, on the communication layer predicates
@@ -164,6 +170,8 @@ let initialize_communication_reqres_proof tr a sender receiver =
 #pop-options
 
 
+(***** Proof for Unauthenticated Request *****)
+
 #push-options "--z3rlimit 250"
 val send_request_proof:
   {|protocol_invariants|} ->
@@ -186,7 +194,7 @@ val send_request_proof:
     | (None, tr_out) -> trace_invariant tr_out
     | (Some (_, req_meta_data), tr_out) -> (
       trace_invariant tr_out /\
-      event_triggered tr_out client (CommClientSendRequest client server request req_meta_data.key <: communication_reqres_event a) /\
+      event_triggered tr_out client (CommClientSendRequest false client server request req_meta_data.key <: communication_reqres_event a) /\
       request == req_meta_data.request /\
       server == req_meta_data.server
     )
@@ -202,7 +210,7 @@ let send_request_proof #invs #a #config #crpreds tr comm_keys_ids  client server
   | (None, tr_out) -> (
     let (key, tr') = mk_rand (AeadKey (comm_layer_aead_tag a) empty) (comm_label client server) 32 tr in
     crpreds.send_request_pred_later tr tr' client server request (get_label tr' key);
-    let ((), tr') = trigger_event client (CommClientSendRequest client server request key <: communication_reqres_event a) tr' in
+    let ((), tr') = trigger_event client (CommClientSendRequest false client server request key <: communication_reqres_event a) tr' in
     let (sid, tr') = new_session_id client tr' in
     let ((), tr') = set_state client sid (ClientSendRequest {server; request=request; key} <: communication_states a) tr' in
     assert(trace_invariant tr');
@@ -211,7 +219,7 @@ let send_request_proof #invs #a #config #crpreds tr comm_keys_ids  client server
   | (Some (_, req_meta_data), tr_out) -> (
     let (key, tr') = mk_rand (AeadKey (comm_layer_aead_tag a) empty) (comm_label client server) 32 tr in
     crpreds.send_request_pred_later tr tr' client server request (get_label tr' key);
-    let ((), tr') = trigger_event client (CommClientSendRequest client server request key <: communication_reqres_event a) tr' in
+    let ((), tr') = trigger_event client (CommClientSendRequest false client server request key <: communication_reqres_event a) tr' in
     let (sid, tr') = new_session_id client tr' in
     let ((), tr') = set_state client sid (ClientSendRequest {server; request; key} <: communication_states a) tr' in
     assert(trace_invariant tr');
@@ -233,7 +241,7 @@ val send_request_properties:
     match send_request com_keys_ids client server request tr with
     | (None, _) -> True
     | (Some (_, req_meta_data), tr_out) -> (
-      event_triggered tr_out client (CommClientSendRequest client server request req_meta_data.key <: communication_reqres_event a) /\
+      event_triggered tr_out client (CommClientSendRequest false client server request req_meta_data.key <: communication_reqres_event a) /\
       server == req_meta_data.server /\
       request == req_meta_data.request
     )
@@ -264,7 +272,7 @@ val receive_request_proof:
     | (None, tr_out) -> trace_invariant tr_out
     | (Some (payload, req_meta_data), tr_out) -> (
       trace_invariant tr_out /\
-      event_triggered tr_out server (CommServerReceiveRequest server payload req_meta_data.key <: communication_reqres_event a) /\
+      event_triggered tr_out server (CommServerReceiveRequest None server payload req_meta_data.key <: communication_reqres_event a) /\
       payload == req_meta_data.request /\
       server == req_meta_data.server
     )
@@ -284,7 +292,7 @@ let receive_request_proof #invs a #config #crpreds tr comm_keys_ids server msg_i
     let Some request = parse a req_msg.request in
 
     let req_msg_bytes:bytes = serialize comm_message_t req_msg_t in
-    let req_send_event client:communication_reqres_event a = CommClientSendRequest client server request req_msg.key in
+    let req_send_event client:communication_reqres_event a = CommClientSendRequest false client server request req_msg.key in
 
     conf_message_properties tr_recv (comm_core_higher_layer_event_preds_reqres a) server req_msg_t;
     
@@ -313,12 +321,12 @@ let receive_request_proof #invs a #config #crpreds tr comm_keys_ids server msg_i
     serialize_parse_inv_lemma #bytes a req_msg.request;
     assert(is_comm_response_payload tr_recv server req_meta_data payload);
 
-    let ((), tr_ev) = trigger_event server (CommServerReceiveRequest server request req_msg.key <: communication_reqres_event a) tr_recv in
+    let ((), tr_ev) = trigger_event server (CommServerReceiveRequest None server request req_msg.key <: communication_reqres_event a) tr_recv in
     let (sid', tr_sess) = new_session_id server tr_ev in
 
     // Needed for the proof to go through
-    assert((state_predicate_communication_layer_reqres a).pred tr_sess server sid' (ServerReceiveRequest {request; key=req_msg.key} <: communication_states a));
-    let ((), tr_st) = set_state server sid' (ServerReceiveRequest {request; key=req_msg.key} <: communication_states a) tr_sess in
+    assert((state_predicate_communication_layer_reqres a).pred tr_sess server sid' (ServerReceiveRequest {client=None; request; key=req_msg.key} <: communication_states a));
+    let ((), tr_st) = set_state server sid' (ServerReceiveRequest {client=None; request; key=req_msg.key} <: communication_states a) tr_sess in
 
     get_response_label_eq_key_label tr_recv req_meta_data;
     
@@ -328,6 +336,179 @@ let receive_request_proof #invs a #config #crpreds tr comm_keys_ids server msg_i
   )
 #pop-options
 
+
+(**** Proof for Authenticated Request ****)
+
+#push-options "--z3rlimit 250"
+val send_request_authenticated_proof:
+  {|protocol_invariants|} ->
+  #a:Type0 -> {|comm_layer_reqres_config a|} ->
+  {|crpreds:comm_reqres_preds a|} ->
+  tr:trace ->
+  comm_keys_ids:communication_keys_sess_ids ->
+  client:principal -> server:principal -> request:a ->
+  Lemma
+  (requires
+    trace_invariant tr /\
+    has_private_keys_invariant /\
+    has_pki_invariant /\
+    has_pki_state_update_invariant /\
+    has_communication_layer_reqres_predicates a /\
+    crpreds.authenticated_request_pred tr client server request (comm_label client server) /\
+    is_well_formed a (is_knowable_by (comm_label client server) tr) request
+  )
+  (ensures (
+    match send_request_authenticated comm_keys_ids client server request tr with
+    | (None, tr_out) -> trace_invariant tr_out
+    | (Some (_, req_meta_data), tr_out) -> (
+      trace_invariant tr_out /\
+      event_triggered tr_out client (CommClientSendRequest true client server request req_meta_data.key <: communication_reqres_event a) /\
+      request == req_meta_data.request /\
+      server == req_meta_data.server
+    )
+  ))
+  [SMTPat (trace_invariant tr);
+  SMTPat (reqres_comm_layer_lemmas_enabled a);
+  SMTPat (send_request_authenticated comm_keys_ids client server request tr)]
+let send_request_authenticated_proof #invs #a #config #crpreds tr comm_keys_ids  client server request =
+  reveal_opaque (`%send_request_authenticated) (send_request_authenticated #a);
+  enable_core_comm_layer_lemmas (comm_core_higher_layer_event_preds_reqres a);
+  let request_bytes = serialize a request in
+  match send_request_authenticated comm_keys_ids client server request tr with
+  | (None, tr_out) -> (
+    let (key, tr') = mk_rand (AeadKey (comm_layer_aead_tag a) empty) (comm_label client server) 32 tr in
+    crpreds.authenticated_request_pred_later tr tr' client server request (get_label tr' key);
+    let ((), tr') = trigger_event client (CommClientSendRequest true client server request key <: communication_reqres_event a) tr' in
+    let (sid, tr') = new_session_id client tr' in
+    let ((), tr') = set_state client sid (ClientSendRequest {server; request; key} <: communication_states a) tr' in
+    assert(trace_invariant tr');
+    ()
+  )
+  | (Some (_, req_meta_data), tr_out) -> (
+    let (key, tr') = mk_rand (AeadKey (comm_layer_aead_tag a) empty) (comm_label client server) 32 tr in
+    crpreds.authenticated_request_pred_later tr tr' client server request (get_label tr' key);
+    let ((), tr') = trigger_event client (CommClientSendRequest true client server request key <: communication_reqres_event a) tr' in
+    let (sid, tr') = new_session_id client tr' in
+    let ((), tr') = set_state client sid (ClientSendRequest {server; request; key} <: communication_states a) tr' in
+    assert(trace_invariant tr');
+    let req_payload:comm_message_t = RequestMessage {request=request_bytes; key} in
+    let (Some msg_id, tr') = send_confidential_authenticated #comm_message_t #(comm_layer_tag_core_config_reqres a) comm_keys_ids client server req_payload tr' in
+    assert(tr_out == tr');
+    assert(trace_invariant tr_out); 
+    ()
+  )
+#pop-options
+
+val send_request_authenticated_properties:
+  #a:eqtype -> {|comm_layer_reqres_config a|} ->
+  tr:trace ->
+  com_keys_ids:communication_keys_sess_ids ->
+  client:principal -> server:principal -> request:a ->
+  Lemma
+  (ensures (
+    match send_request_authenticated com_keys_ids client server request tr with
+    | (None, _) -> True
+    | (Some (_, req_meta_data), tr_out) -> (
+      event_triggered tr_out client (CommClientSendRequest true client server request req_meta_data.key <: communication_reqres_event a) /\
+      server == req_meta_data.server /\
+      request == req_meta_data.request
+    )
+  ))
+let send_request_authenticated_properties #a #config tr com_keys_ids client server request =
+  reveal_opaque (`%send_request_authenticated) (send_request_authenticated #a);
+  ()
+
+
+#push-options "--z3rlimit 75"
+val receive_request_authenticated_proof:
+  {|invs:protocol_invariants|} ->
+  a:Type -> {|comm_layer_reqres_config a|} ->
+  {|crpreds:comm_reqres_preds a|} ->
+  tr:trace ->
+  comm_keys_ids:communication_keys_sess_ids ->
+  server:principal -> msg_id:timestamp ->
+  Lemma
+  (requires
+    invs.crypto_invs.usages == default_crypto_usages /\
+    trace_invariant tr /\
+    has_private_keys_invariant /\
+    has_pki_invariant /\
+    has_communication_layer_reqres_predicates a
+  )
+  (ensures (
+    match receive_request_authenticated #a comm_keys_ids server msg_id tr with
+    | (None, tr_out) -> trace_invariant tr_out
+    | (Some (payload, req_meta_data), tr_out) -> (
+      trace_invariant tr_out /\
+      event_triggered tr_out server (CommServerReceiveRequest req_meta_data.client server payload req_meta_data.key <: communication_reqres_event a) /\
+      payload == req_meta_data.request /\
+      server == req_meta_data.server
+    )
+  ))
+  [SMTPat (trace_invariant tr);
+  SMTPat (reqres_comm_layer_lemmas_enabled a);
+  SMTPat (receive_request_authenticated #a comm_keys_ids server msg_id tr)]
+let receive_request_authenticated_proof #invs a #config #crpreds tr comm_keys_ids server msg_id =
+  reveal_opaque (`%receive_request_authenticated) (receive_request_authenticated #a);
+  enable_core_comm_layer_lemmas (comm_core_higher_layer_event_preds_reqres a);
+  match receive_request_authenticated #a comm_keys_ids server msg_id tr with
+  | (None, tr_out) -> ()
+  | (Some (payload, req_meta_data), tr_out) -> (
+    receive_confidential_authenticated_proof #invs #comm_message_t #(comm_layer_tag_core_config_reqres a) tr (comm_core_higher_layer_event_preds_reqres a) comm_keys_ids server msg_id;
+    let (Some cm, tr_recv) = receive_confidential_authenticated #comm_message_t #(comm_layer_tag_core_config_reqres a) comm_keys_ids server msg_id tr in
+    assert(trace_invariant tr_recv);
+    let RequestMessage req_msg = cm.payload in
+    let Some request = parse a req_msg.request in
+
+    let req_msg_bytes:bytes = serialize comm_message_t cm.payload in
+    let req_send_event:communication_reqres_event a = CommClientSendRequest true cm.sender server request req_msg.key in
+
+    confauth_message_properties' tr_recv (comm_core_higher_layer_event_preds_reqres a) cm.sender server cm.payload;
+    
+    // Properties that can be proved uniformly in both the honest and corrupt case
+    eliminate event_triggered tr_recv cm.sender req_send_event \/ is_well_formed (comm_message_t) (is_publishable tr_recv) cm.payload
+    returns (
+      is_well_formed a (is_knowable_by (get_label tr_recv req_meta_data.key) tr_recv) request /\
+      req_msg.key `has_usage tr_recv` (AeadKey (comm_layer_aead_tag a) empty)
+    )
+    with _. (
+      get_response_label_eq_key_label tr_recv req_meta_data;
+
+      let i = find_event_triggered_at_timestamp tr_recv cm.sender req_send_event in
+      assert(event_predicate_communication_layer_reqres a (prefix tr_recv i) cm.sender req_send_event);
+      ()
+    )
+    and _. (has_usage_publishable tr_recv req_msg.key (AeadKey (comm_layer_aead_tag a) empty);
+      parse_wf_lemma a (is_publishable tr_recv) req_msg.request;
+      ()
+    );
+    
+    confauth_message_properties tr_recv (comm_core_higher_layer_event_preds_reqres a) cm.sender server cm.payload;
+    assert((event_predicate_communication_layer_reqres a) tr_recv server (CommServerReceiveRequest (Some cm.sender) server request req_msg.key <: communication_reqres_event a)) by (
+      let open FStar.Tactics in
+      norm [delta_only [`%event_predicate_communication_layer_reqres]; iota];
+      dump "";
+      //admit_all ();
+      ()
+    );
+    let ((), tr_ev) = trigger_event server (CommServerReceiveRequest (Some cm.sender) server request req_msg.key <: communication_reqres_event a) tr_recv in
+    assert(trace_invariant tr_ev);
+    let (sid', tr_sess) = new_session_id server tr_ev in
+
+    // Needed for the proof to go through
+    assert((state_predicate_communication_layer_reqres a).pred tr_sess server sid' (ServerReceiveRequest {client=Some cm.sender; request; key=req_msg.key} <: communication_states a));
+    let ((), tr_st) = set_state server sid' (ServerReceiveRequest {client=Some cm.sender; request; key=req_msg.key} <: communication_states a) tr_sess in
+
+    get_response_label_eq_key_label tr_recv req_meta_data;
+    
+    assert(tr_out == tr_st);
+    assert(trace_invariant tr_out);
+    ()
+  )
+#pop-options
+
+
+(**** Proof for Response ****)
 
 val mk_comm_layer_response_nonce_proof:
   {|protocol_invariants|} ->
@@ -385,7 +566,7 @@ let mk_comm_layer_response_nonce_labeled_proof #invs #a tr req_meta_data usg lab
   reveal_opaque (`%get_response_label) (get_response_label);
   ()
 
-
+#push-options "--ifuel 1 --z3rlimit 20"
 val compute_response_message_proof:
   {|crypto_invariants|} ->
   #a:Type0 -> {|comm_layer_reqres_config a|} ->
@@ -399,7 +580,7 @@ val compute_response_message_proof:
     is_well_formed a (is_knowable_by (get_response_label tr req_meta_data) tr) response /\
     is_publishable tr nonce /\
     req_meta_data.key `has_usage tr` (AeadKey (comm_layer_aead_tag a) empty) /\
-    event_triggered tr server (CommServerSendResponse server request response req_meta_data.key <: communication_reqres_event a)
+    event_triggered tr server (CommServerSendResponse req_meta_data.client server request response req_meta_data.key <: communication_reqres_event a)
   )
   (ensures
     is_publishable tr (compute_response_message #a server req_meta_data nonce response)
@@ -409,7 +590,7 @@ let compute_response_message_proof #cinvs #a tr server req_meta_data nonce reque
   get_response_label_eq_key_label tr req_meta_data;
   let res_bytes = serialize a response in
   serialize_wf_lemma a (is_knowable_by (get_response_label tr req_meta_data) tr) response;
-  let ad:authenticated_data = {server} in
+  let ad:authenticated_data = {client=req_meta_data.client; server} in
   let ad_bytes = serialize authenticated_data ad in
   serialize_wf_lemma authenticated_data (is_publishable tr) ad;
   let ciphertext = aead_enc req_meta_data.key nonce res_bytes ad_bytes in
@@ -417,6 +598,7 @@ let compute_response_message_proof #cinvs #a tr server req_meta_data nonce reque
   FStar.Classical.move_requires (aead_enc_preserves_publishability tr req_meta_data.key nonce res_bytes) ad_bytes;
   serialize_wf_lemma comm_message_t (is_publishable tr) (ResponseMessage {nonce; ciphertext});
   ()
+#pop-options
 
 #push-options "--z3rlimit 10"
 val send_response_proof:
@@ -429,7 +611,7 @@ val send_response_proof:
   (requires
     trace_invariant tr /\
     has_communication_layer_reqres_predicates a /\
-    event_triggered tr server (CommServerReceiveRequest server req_meta_data.request req_meta_data.key <: communication_reqres_event a) /\
+    event_triggered tr server (CommServerReceiveRequest req_meta_data.client server req_meta_data.request req_meta_data.key <: communication_reqres_event a) /\
     crpreds.send_response_pred tr server req_meta_data.request response (get_response_label tr req_meta_data) /\
     is_well_formed a (is_knowable_by (get_response_label tr req_meta_data) tr) response
   )
@@ -448,7 +630,7 @@ let send_response_proof #invs #a #config #crpreds tr server req_meta_data respon
     let (Some state, tr_st):(option (communication_states a) & trace) = get_state server req_meta_data.sid tr in
     let ServerReceiveRequest srr = state in
     assert(trace_invariant tr_st);
-    let ((), tr_ev) = trigger_event server (CommServerSendResponse server req_meta_data.request response req_meta_data.key <: communication_reqres_event a) tr_st in
+    let ((), tr_ev) = trigger_event server (CommServerSendResponse req_meta_data.client server req_meta_data.request response req_meta_data.key <: communication_reqres_event a) tr_st in
     get_response_label_eq_key_label tr_ev req_meta_data;
     assert(trace_invariant tr_ev);
     let (nonce, tr_nonce) = mk_rand NoUsage public 32 tr_ev in
@@ -463,40 +645,40 @@ let send_response_proof #invs #a #config #crpreds tr server req_meta_data respon
 #pop-options
 
 
-#push-options "--z3rlimit 50"
+#push-options "--ifuel 1 --z3rlimit 50"
 val decode_response_proof:
   {|crypto_invariants|} ->
   #a:Type -> {|comm_layer_reqres_config a|} ->
   tr:trace ->
   client:principal -> server:principal ->
-  response_bytes:bytes -> key:bytes ->
+  response_bytes:bytes -> req_meta_data:comm_meta_data a ->
   Lemma
   (requires
     has_communication_layer_reqres_crypto_predicates a /\
     is_publishable tr response_bytes /\
-    is_secret (comm_label client server) tr key /\
-    key `has_usage tr` (AeadKey (comm_layer_aead_tag a) empty)
+    is_secret (comm_label client server) tr req_meta_data.key /\
+    req_meta_data.key `has_usage tr` (AeadKey (comm_layer_aead_tag a) empty)
   )
   (ensures (
-    match decode_response_message server key response_bytes with
+    match decode_response_message server req_meta_data.key response_bytes req_meta_data with
     | None -> True
     | Some response -> (
-      is_well_formed a (is_knowable_by (get_label tr key) tr) response /\
-      is_knowable_by (get_label tr key) tr (serialize a response) /\
-      ((exists request. event_triggered tr server (CommServerSendResponse server request response key <: communication_reqres_event a))
+      is_well_formed a (is_knowable_by (get_label tr req_meta_data.key) tr) response /\
+      is_knowable_by (get_label tr req_meta_data.key) tr (serialize a response) /\
+      ((exists request. event_triggered tr server (CommServerSendResponse req_meta_data.client server request response req_meta_data.key <: communication_reqres_event a))
         \/ is_corrupt tr (principal_label client) \/ is_corrupt tr (principal_label server))
     )
   ))
-let decode_response_proof #invs #a tr client server response_bytes key =
+let decode_response_proof #invs #a tr client server response_bytes req_meta_data =
   reveal_opaque (`%decode_response_message) (decode_response_message #a);
-  match decode_response_message #a server key response_bytes with
+  match decode_response_message #a server req_meta_data.key response_bytes req_meta_data with
   | None -> ()
   | Some response -> (
     parse_wf_lemma comm_message_t (is_publishable tr) response_bytes;
     let Some (ResponseMessage {nonce; ciphertext}) = parse comm_message_t response_bytes in
-    serialize_wf_lemma authenticated_data (is_publishable tr) {server};
-    let ad_bytes = serialize authenticated_data {server} in
-    let Some res_bytes = aead_dec key nonce ciphertext ad_bytes in
+    serialize_wf_lemma authenticated_data (is_publishable tr) {client=req_meta_data.client; server};
+    let ad_bytes = serialize authenticated_data {client=req_meta_data.client; server} in
+    let Some res_bytes = aead_dec req_meta_data.key nonce ciphertext ad_bytes in
     serialize_parse_inv_lemma a res_bytes;
     ()
   )
@@ -507,21 +689,21 @@ val comm_client_send_request_injective:
   {|protocol_invariants|} ->
   #a:Type -> {| comm_layer_reqres_config a |} ->
   {|crpreds:comm_reqres_preds a|} ->
-  tr:trace ->
+  tr:trace -> authenticated:bool ->
   client:principal -> client':principal -> server:principal ->
   request:a -> request':a -> key:bytes ->
   Lemma
   (requires
     trace_invariant tr /\
     has_communication_layer_reqres_predicates a /\
-    event_triggered tr client' (CommClientSendRequest client' server request' key <: communication_reqres_event a) /\
-    event_triggered tr client (CommClientSendRequest client server request key <: communication_reqres_event a)
+    event_triggered tr client' (CommClientSendRequest authenticated client server request' key <: communication_reqres_event a) /\
+    event_triggered tr client (CommClientSendRequest authenticated client server request key <: communication_reqres_event a)
   )
   (ensures
     client == client' /\
     request == request'
   )
-let comm_client_send_request_injective #invs #a #config #crpreds tr client client' server request request' key = ()
+let comm_client_send_request_injective #invs #a #config #crpreds tr authenticated client client' server request request' key = ()
 #pop-options
 
 #push-options "--z3rlimit 100"
@@ -531,47 +713,77 @@ val request_response_property:
   {|comm_reqres_preds a|} ->
   tr:trace ->
   client:principal -> server:principal ->
-  request:a -> response:a -> key:bytes ->
+  request:a -> response:a ->
+  req_meta_data:comm_meta_data a ->
   Lemma
   (requires
     trace_invariant tr /\
     has_communication_layer_reqres_predicates a /\
-    event_triggered tr client (CommClientSendRequest client server request key <: communication_reqres_event a) /\
-    is_secret (comm_label client server) tr key /\
-    key `has_usage tr` (AeadKey (comm_layer_aead_tag a) empty) /\
-    (exists request'. event_triggered tr server (CommServerSendResponse server request' response key <: communication_reqres_event a)
+    event_triggered tr client (CommClientSendRequest (Some? req_meta_data.client) client server request req_meta_data.key <: communication_reqres_event a) /\
+    is_secret (comm_label client server) tr req_meta_data.key /\
+    req_meta_data.key `has_usage tr` (AeadKey (comm_layer_aead_tag a) empty) /\
+    (match req_meta_data.client with
+    | None -> true
+    | Some client' ->  client = client') /\
+    (exists request'. event_triggered tr server (CommServerSendResponse req_meta_data.client server request' response req_meta_data.key <: communication_reqres_event a)
         \/ is_corrupt tr (principal_label client) \/ is_corrupt tr (principal_label server))
   )
   (ensures
     (
-      event_triggered tr server (CommServerSendResponse server request response key <: communication_reqres_event a) /\
-      event_triggered tr server (CommServerReceiveRequest server request key <: communication_reqres_event a)
+      event_triggered tr server (CommServerSendResponse req_meta_data.client server request response req_meta_data.key <: communication_reqres_event a) /\
+      event_triggered tr server (CommServerReceiveRequest req_meta_data.client server request req_meta_data.key <: communication_reqres_event a)
     ) \/ is_corrupt tr (principal_label client) \/ is_corrupt tr (principal_label server)
   )
-let request_response_property #invs #a #config #crpreds tr client server request response key =
-  let send_event request:communication_reqres_event a = CommServerSendResponse server request response key in
-  introduce (~(is_corrupt tr (principal_label client) \/ is_corrupt tr (principal_label server))) ==> (exists request'. event_triggered #(communication_reqres_event a) #(event_communication_reqres_event #a #config) tr server (CommServerSendResponse server request' response key <: communication_reqres_event a)) 
+let request_response_property #invs #a #config #crpreds tr client server request response req_meta_data =
+  let send_event request:communication_reqres_event a = CommServerSendResponse req_meta_data.client server request response req_meta_data.key in
+  introduce (~(is_corrupt tr (principal_label client) \/ is_corrupt tr (principal_label server))) ==> 
+    (exists request'. event_triggered #(communication_reqres_event a) #(event_communication_reqres_event #a #config) tr server (CommServerSendResponse req_meta_data.client server request' response req_meta_data.key <: communication_reqres_event a)) 
   with _. (
-    eliminate exists request'. event_triggered tr server (CommServerSendResponse server request' response key <: communication_reqres_event a)
-    returns event_triggered tr server (CommServerSendResponse server request response key <: communication_reqres_event a) /\
-            event_triggered tr server (CommServerReceiveRequest server request key <: communication_reqres_event a)
+    eliminate exists request'. event_triggered tr server (CommServerSendResponse req_meta_data.client server request' response req_meta_data.key <: communication_reqres_event a)
+    returns event_triggered tr server (CommServerSendResponse req_meta_data.client server request response req_meta_data.key <: communication_reqres_event a) /\
+            event_triggered tr server (CommServerReceiveRequest req_meta_data.client server request req_meta_data.key <: communication_reqres_event a)
     with _. (
       let j = find_event_triggered_at_timestamp tr server (send_event request') in
       assert((event_predicate_communication_layer_reqres a) (prefix tr j) server (send_event request'));
-      assert((exists client'. 
-        event_triggered tr client' (CommClientSendRequest client' server request' key <: communication_reqres_event a)));
-      eliminate exists client'. event_triggered tr client' (CommClientSendRequest client' server request' key <: communication_reqres_event a)
-      returns event_triggered tr server (CommServerSendResponse server request response key <: communication_reqres_event a) /\
-              event_triggered tr server (CommServerReceiveRequest server request key <: communication_reqres_event a)
-      with _. (
-        comm_client_send_request_injective tr client client' server request request' key;
-        ()
+      assert(event_triggered tr server (CommServerReceiveRequest req_meta_data.client server request' req_meta_data.key <: communication_reqres_event a));
+      match req_meta_data.client with
+      | None -> (
+        assert((exists client'. 
+          event_triggered tr client' (CommClientSendRequest (Some? req_meta_data.client) client' server request' req_meta_data.key <: communication_reqres_event a)));
+        eliminate exists client'. event_triggered tr client' (CommClientSendRequest (Some? req_meta_data.client) client' server request' req_meta_data.key <: communication_reqres_event a)
+        returns event_triggered tr server (CommServerSendResponse req_meta_data.client server request response req_meta_data.key <: communication_reqres_event a) /\
+                event_triggered tr server (CommServerReceiveRequest req_meta_data.client server request req_meta_data.key <: communication_reqres_event a)
+        with _. (
+          comm_client_send_request_injective tr (Some? req_meta_data.client) client client' server request request' req_meta_data.key;
+          ()
+        )
+      )
+      | Some client'' -> (
+        assert(client'' == client);
+        assert(
+          event_triggered tr client (CommClientSendRequest true client server request' req_meta_data.key <: communication_reqres_event a) \/
+          is_corrupt tr (long_term_key_label client)
+        );
+        //assert((principal_label client) `can_flow tr` (long_term_key_label client));
+        eliminate  event_triggered tr client (CommClientSendRequest true client server request' req_meta_data.key <: communication_reqres_event a) \/ is_corrupt tr (long_term_key_label client)
+        returns _
+        with _. (
+          comm_client_send_request_injective tr true client client server request request' req_meta_data.key;
+          ()
+        )
+        and _. (
+          assert((principal_label client) `can_flow tr` (long_term_key_label client));
+          assert(is_corrupt tr (principal_label client));
+          //assert(~(is_corrupt tr (principal_label client)));
+          //admit();
+          ()
+        )
       )
     )
   )
 #pop-options
 
-#push-options "--z3rlimit 150"
+#push-options "--z3rlimit 250"
 val receive_response_proof:
   {|protocol_invariants|} ->
   #a:Type -> {|comm_layer_reqres_config a|} ->
@@ -582,14 +794,15 @@ val receive_response_proof:
   (requires
     trace_invariant tr /\
     has_communication_layer_reqres_predicates a /\
-    event_triggered tr client (CommClientSendRequest client req_meta_data.server req_meta_data.request req_meta_data.key <: communication_reqres_event a)
+    // TODO shouldn't this be put into the state invariant?
+    event_triggered tr client (CommClientSendRequest (Some? req_meta_data.client) client req_meta_data.server req_meta_data.request req_meta_data.key <: communication_reqres_event a)
   )
   (ensures (
     match receive_response client req_meta_data msg_id tr with
     | (None, tr_out) -> trace_invariant tr_out
     | (Some (payload, _), tr_out) -> (
       trace_invariant tr_out /\
-      event_triggered tr_out client (CommClientReceiveResponse client req_meta_data.server req_meta_data.request payload req_meta_data.key <: communication_reqres_event a)
+      event_triggered tr_out client (CommClientReceiveResponse (Some? req_meta_data.client) client req_meta_data.server req_meta_data.request payload req_meta_data.key <: communication_reqres_event a)
     )
   ))
   [SMTPat (trace_invariant tr);
@@ -600,18 +813,40 @@ let receive_response_proof #invs #a #crpreds tr client req_meta_data msg_id =
   match receive_response #a client req_meta_data msg_id tr with
   | (None, tr_out) -> ()
   | (Some (response, _), tr_out) -> (
-    let server = req_meta_data.server in
-    let key = req_meta_data.key in
     let (Some state, tr'):(option (communication_states a) & trace) = get_state client req_meta_data.sid tr in
     let ClientSendRequest csr = state in
+    let server = csr.server in
+    let key = csr.key in
     let (Some resp_msg_bytes, tr') = recv_msg msg_id tr' in
-    decode_response_proof #invs.crypto_invs #a tr' client server resp_msg_bytes key;
-    let Some response = decode_response_message server key resp_msg_bytes in
-    request_response_property tr' client server req_meta_data.request response key;
-    get_response_label_eq_key_label tr' req_meta_data;
-    let ((), tr') = set_state client req_meta_data.sid (ClientReceiveResponse {server=csr.server; response; key=csr.key} <: communication_states a) tr' in
-    let ((), tr') = trigger_event client (CommClientReceiveResponse client csr.server req_meta_data.request response csr.key <: communication_reqres_event a) tr' in
-    assert(event_triggered tr' client (CommClientReceiveResponse client csr.server req_meta_data.request response csr.key <: communication_reqres_event a));
+    decode_response_proof #invs.crypto_invs #a tr' client server resp_msg_bytes req_meta_data;
+    let Some response = decode_response_message server key resp_msg_bytes req_meta_data in
+    request_response_property tr' client server req_meta_data.request response req_meta_data;
+    assert(
+      match req_meta_data.client with
+    | None -> true
+    | Some client' ->  client = client'
+    );
+    //assert(req_meta_data.client == (if (Some? req_meta_data.client) then Some client else None));
+    //admit();
+    assert(
+      event_triggered tr' server (CommServerSendResponse (if (Some? req_meta_data.client) then Some client else None) server req_meta_data.request response key <: communication_reqres_event a) \/
+        is_corrupt tr' (principal_label client) \/ is_corrupt tr' (principal_label server)
+    );
+    //admit();
+    //get_response_label_eq_key_label tr' req_meta_data;
+    let ((), tr') = set_state client req_meta_data.sid (ClientReceiveResponse {server; response; key} <: communication_states a) tr' in
+    assert(trace_invariant tr');
+    //admit();
+    let ((), tr') = trigger_event client (CommClientReceiveResponse (Some? req_meta_data.client) client server req_meta_data.request response key <: communication_reqres_event a) tr' in
+    assert(event_triggered tr' client (CommClientSendRequest (Some? req_meta_data.client) client server req_meta_data.request key <: communication_reqres_event a));
+    //admit();
+    assert((event_predicate_communication_layer_reqres a) tr' client (CommClientReceiveResponse (Some? req_meta_data.client) client server req_meta_data.request response key <: communication_reqres_event a)) by (
+      let open FStar.Tactics in
+      norm [delta_only [`%event_predicate_communication_layer_reqres]; iota];
+      dump "";
+      //admit_all ();
+      ()
+    );
     assert(tr_out == tr');
     assert(trace_invariant tr_out);
     ()
